wip

code/rocq/elpi.v
@@ -8,15 +8,15 @@ Import Language.
 Module Nur (U : Unif).
 
   Module RunP := RunP(U).
-  Import RunP Run U Language.
+  Import RunP Run Language.
 
   Inductive G := 
     | call : Tm -> G
     | cut : list (list G) -> G
-    (* | fail : G *)
+    | fail : G
     .
-  derive G.
-  HB.instance Definition _ := hasDecEq.Build state state_eqb_OK.
+  #[verbose]derive G.
+  HB.instance Definition _ := hasDecEq.Build G G_eqb_OK.
 
   Definition alt := (list G).
 
@@ -37,8 +37,8 @@ Module Nur (U : Unif).
         nur p s [::call t & gl] a s1 r
   | FailE p s s1 t gl a al r : 
     F p t s = [::] -> nur p s a al s1 r -> nur p s [::call t & gl] (a :: al) s1 r
-  (* | FailE1 p s s1 gl a al r :  *)
-    (* nur p s a al s1 r -> nur p s [::fail & gl] (a :: al) s1 r. *)
+  | FailE1 p s s1 gl a al r : 
+    nur p s a al s1 r -> nur p s [::fail & gl] (a :: al) s1 r
   .
 
   Lemma nur_consistent {p s G x xs1 xs2 s1 s2} :
@@ -56,15 +56,15 @@ Module Nur (U : Unif).
       apply: IH.
       inversion H2; subst => //.
       congruence.
-    (* - move=> p1 s1 s2 gl a al r H IH xs2 s3 H2.
+    - move=> p1 s1 s2 gl a al r H IH xs2 s3 H2.
       apply: IH.
-      by inversion H2; subst. *)
+      by inversion H2; subst.
   Qed.
 
   Definition add_ca gl (l2 : list alt) : G :=
     match gl with
     | call _ => gl 
-    (* | fail => gl *)
+    | fail => gl
     | cut l1 => cut (l1 ++ l2) end.
   
   Definition add_cas lA lB : alt :=
@@ -77,11 +77,15 @@ Module Nur (U : Unif).
     else [::]
     .
 
+  Definition normalize_aux (l : list G) : list G :=
+    if (fail: G) \in l then [::fail] else l.
+  
+  Definition normalize := map normalize_aux.
+
   Fixpoint state_to_list (A: state) (bt : list alt) : list alt :=
     match A with
     | OK | Top => [::[::]]
-    | KO 
-    (* => [::[::fail]] *)
+    | KO => [::[::fail]]
     | Dead => [::]
     | Goal _ Cut => [::[::cut [::]]]
     | Goal _ (Call t) => [::[::call t]]
@@ -90,8 +94,8 @@ Module Nur (U : Unif).
       let lA := state_to_list A (lB ++ bt) in
       [seq add_cas la bt | la <- lA] ++ lB
     | And A B0 B => 
-      let lA := state_to_list A bt in
-      let lB := state_to_list B bt in
+      let lA   := state_to_list A bt in
+      let lB   := state_to_list B bt in
       let lB0 := state_to_list B0 bt in
       (* if failed A then add_alt lB0 lA lB0 
       else add_alt lB0 lA lB  *)
@@ -108,7 +112,9 @@ Module Nur (U : Unif).
       [:: call x; call w];
       [:: call y; call a]].
   Proof.
-    move=>/=. by [].
+    move=>/=.
+    rewrite /normalize_aux/=.
+    by [].
   Qed.
 
   Goal forall p z w s1 s2 a, 
@@ -117,9 +123,25 @@ Module Nur (U : Unif).
       And 
         (Or OK s1 KO) (f a) 
         (Or (f z) s2 (f w))) [::] = 
-      [:: [:: call z]; [:: call w]].
+      [:: [:: call z]; [:: call w]; [:: fail; call a]].
   Proof.
-    move=>/=. by [].
+    move=>/=.
+    rewrite /normalize_aux/=.
+    by [].
+  Qed.
+
+  (* THIS IS IMPORTANT *)
+  Goal forall p s1 s2 a b c d, 
+    let f x := (Goal p (Call x)) in
+    state_to_list (
+      And 
+        (Or KO s1 (f a)) (f b) 
+        (Or (f c) s2 (f d))) [::] = 
+      [:: [:: fail; call c]; [:: fail; call d]; [:: call a; call b]].
+  Proof.
+    move=>/=.
+    rewrite /normalize_aux/=.
+    by [].
   Qed.
 
   Goal forall p a b s1 s2, 
@@ -138,23 +160,26 @@ Module Nur (U : Unif).
      [:: [:: call c; cut [:: [:: call b]]]; [:: call a]; [:: call b]].
   Proof. by []. Qed.
 
-  Definition nur' r1 A l s :=
+  Definition state_to_list_cons A :=
+    forall l, exists x xs, state_to_list A l = x :: xs.
+
+  Definition nur' r1 A l s s1 :=
     forall x xs, state_to_list A l = x :: xs ->
-        forall p, exists s1, nur p s x xs s1 r1.
+        forall p, nur p s x xs s1 r1.
 
   Definition runElpi A :=
     forall s B s1 b,
       runb s A s1 B b -> 
-          forall l, exists r1, nur' r1 A l s /\ state_to_list B l = r1.
+        forall l, exists r1, nur' r1 A l s s1 /\ state_to_list B l = r1.
   
   Goal @runElpi OK.
   Proof.
-    rewrite/runElpi/nur'.
-    inversion 1; subst => //=; inversion H1 => //p; subst.
-    case: H7 => _ <-/=.
+    rewrite/runElpi/nur' => s B s1 b H.
+    inversion H; clear H; subst => //=; inversion H0 => //p; subst.
+    case: H6 => <- <-/=.
     eexists; split; [|reflexivity].
-    move=> ??[<-<-].
-    eexists. apply: StopE.
+    move=> ??[<-<-]?.
+    apply: StopE.
   Qed.
   
   Goal @runElpi KO.
@@ -173,8 +198,8 @@ Module Nur (U : Unif).
       case: H2 => ??; subst.
       inversion H3; subst => //.
       case: H8 => ??; subst => /=.
-      eexists; split => //??[<-<-].
-      eexists;apply: StopE.
+      eexists; split => //??[<-<-]?.
+      apply: StopE.
     - inversion H1; subst => //.
       case: H4 => ??;subst.
       inversion H5 => //.
@@ -190,19 +215,22 @@ Module Nur (U : Unif).
     inversion H2.
   Qed.
 
-  Lemma state_to_list_cutr {A l} : state_to_list (cutr A) l = [::].
+  (* Lemma state_to_list_cutr {A l} : state_to_list (cutr A) l = nseq n [::fail].
   Proof.
     elim: A l => //.
     + move=> A HA s B HB /= l.
       by rewrite HB HA cats0/=.
     + move=> A HA B0 HB0 B HB /= l.
       by rewrite HA HB HB0.
-  Qed.
+  Qed. *)
 
   Lemma state_to_list_dead {A l}: state_to_list (dead A) l = [::].
   Proof.
-    rewrite -cutr_dead_is_dead.
-    apply: state_to_list_cutr.
+    elim: A l => //.
+    - move=> A HA s B HB/= l.
+      by rewrite HB HA.
+    - move=> A HA B0 HB0 B HB l /=.
+      by rewrite HB0 HA HB.
   Qed.
 
   Lemma flatten_empty {T R : Type} {l: list T}:
@@ -239,7 +267,8 @@ Module Nur (U : Unif).
         move=>[A'[HA'->]]/=.
         by rewrite (HA _ _ _ _ HA').
       move=> [B'[dA[HB' ->]]].
-      rewrite dA/=; rewrite !state_to_list_dead/=; apply: HB HB'.
+      rewrite dA/=; rewrite !state_to_list_dead/=.
+      apply: HB HB'.
     - move=> A HA B0 _ B HB s1 C s2 l.
       move=>/simpl_expand_and_solved[s'[A'[B'[HA'[HB'->]]]]]/=.
       by rewrite (HA _ _ _ _ HA')(HB _ _ _ _ HB').
@@ -261,212 +290,211 @@ Module Nur (U : Unif).
     by move=>/success_state_to_list->[].
   Qed.
 
-  Lemma expand_state_to_list {A s r}:
-    expand s A = r -> is_fail r == false ->
-      forall {l}, exists x xs, state_to_list A l = x :: xs.
+  Lemma failed_state_to_list {A}:
+    failed A = false -> state_to_list_cons A.
   Proof.
-    elim: A s r => //; try by move=> s r <- //; do 2 eexists.
-    - by move=> p [|t] s r<-//=; do 2 eexists.
-    - move=> A HA s B HB s1 r.
-      case: r => // s2 C.
-      - move=>/simpl_expand_or_expanded[].
-          move=> [A'[dA[HA'->]]] _ l/=.
-          have:= HA _ _ HA' isT (state_to_list B l ++ l).
-          move=> [y[ys ->]]; by do 2 eexists.
-        move=>[].
-          move=>[A'[dA[HA'->]]] _ l /=.
-          have:= HA _ _ HA' isT (state_to_list B l ++ l).
-          move=> [y[ys ->]]; by do 2 eexists.
-        move=> [-> [B' [+ ->]]] _ l /=.
-        rewrite state_to_list_dead/=.
-        move=> []H; apply: HB H isT _.
-      - move=> /simpl_expand_or_cut[D [-> [H ->]]] _ l/=.
-        rewrite state_to_list_dead/=.
-      - apply: HB H isT _.
-      - move=> /simpl_expand_or_solved[].
-          move=>[A'[HA'->]] _ l/=.
-          have:= success_state_to_list (proj1 (expand_solved_success HA')).
-          move=> ->/=.
-          by do 2 eexists.
-        move=> [B'[->[HB'->]]] _ l/=.
-        rewrite state_to_list_dead/=.
-        apply: HB HB' isT _.
-    - move=> A HA B0 _ B HB s r.
-      case: r => // s2 C.
-      - move=> /simpl_expand_and_expanded[].
-          move=>[A'[HA'->]] _ l/=.
-          have:= HA _ _ HA' isT l.
-          move=>[x [xs]]->/=.
-  Abort.
+    elim: A => //.
+    - move=> /=. by move=> /=; do 2 eexists.
+    - by move=> /=; do 2 eexists.
+    - by move=> p []//=; do 2 eexists.
+    - move=> A HA s B HB/=+l.
+      case: ifP => /eqP.
+        move=>->/HB -/(_ l)/= [x[xs]]->/=.
+        rewrite state_to_list_dead; by do 2 eexists.
+      move=> dA /HA-/(_ (state_to_list B l ++ l))[x [xs]]/=->.
+      by do 2 eexists.
+    - move=> A HA B0 _ B HB/= + l/=.
+      case fA: failed => //.
+      have [x[xs]]:= HA fA l => ->.
+      move=>/HB-/(_ l)[w[ws]]->; by do 2 eexists.
+  Qed.
 
-  Lemma expandedb_state_to_list {A s B s1 b}:
+  Lemma expandedb_done_state_to_list {A s B s1 b}:
     expandedb s A (Done s1 B) b ->
-      forall {l}, exists x xs, state_to_list A l = x :: xs.
+      state_to_list_cons A.
   Proof.
-    remember (Done _ _) as d eqn:Hd => H.
-    elim: H B s1 Hd; clear => //.
-    - move=> s s' A B H C s1 [_ _] l.
-      have:= success_state_to_list (proj1 (expand_solved_success H)).
-      by move=>->; do 2 eexists.
-    - move=> s s' r A B b HA HB IH B'  s2 ? l; subst.
-      have {}IH := IH _ _ erefl.
-      move: HA HB IH.
+    move=>/expandedb_Done_not_failed.
+    by move=> /failed_state_to_list.
+  Qed.
 
-  Abort.
+  Lemma next_alt_state_to_list {s1 A s2 B}:
+    next_alt s1 A = Some (s2, B) -> state_to_list_cons B.
+  Proof.
+    rewrite /state_to_list_cons.
+    elim: A s1 B s2 => //.
+    - move=> A HA s B HB s1 C s2/=.
+      case: ifP => /eqP.
+        move=>->.
+        case X: next_alt => [[s3 D]|]//.
+        move=>[_ <-]l/=.
+        rewrite state_to_list_dead/=.
+        apply: HB X _.
+      case X: next_alt => [[s3 D]|] dA.
+        move=> [_ <-]l/=.
+        have [x [xs]]:= HA _ _ _ X (state_to_list B l ++ l).
+        move=>->; by do 2 eexists.
+      case: ifP => /eqP// dB.
+      case: ifP => // fB.
+        case Y : next_alt => [[s3 D]|]//.
+        move=> [_<-]l/=.
+        rewrite state_to_list_dead/=.
+        apply: HB Y _.
+      move=>[_<-]l/=.
+      have [x[xs]]:= @failed_state_to_list _ fB l.
+      move=>->/=.
+      rewrite state_to_list_dead/=.
+      by do 2 eexists.
+    - move=> A HA B0 _ B HB s1 C s2/=.
+      case: ifP => /eqP//dA.
+      case: ifP => //fA.
+        case X: next_alt => [[s3 D]|]//.
+        case: ifP => //fB0[_<-]/=l.
+        have [x[xs]]:= HA _ _ _ X l => ->.
+        have [y[ys]]:= @failed_state_to_list _ fB0 l => ->.
+        by do 2 eexists.
+      case X: next_alt =>[[s3 D]|]//.
+        move=>[_<-]l/=.
+        have [x[xs]]:= @failed_state_to_list _ fA l => ->.
+        have [y[ys]]:= HB _ _ _ X l=>->.
+        by do 2 eexists.
+      case Y: next_alt => [[s3 D]|]//.
+      case: ifP => //fB0[_<-]l/=.
+      have [x[xs]]:= @failed_state_to_list _ fB0 l => ->.
+      have [y[ys]]:= HA _ _ _ Y l=>->.
+      by do 2 eexists.
+  Qed.
+
+  (* Lemma expandedb_fail_state_to_list {s A B b1 s' C}:
+    expandedb s A (Failed B) b1 -> next_alt s B = Some (s', C) -> 
+      state_to_list_cons A.
+  Proof.
+    remember (Failed _) as f eqn:Hf => H.
+    elim: H B Hf => //; clear.
+    - move=> s A B HA ? [] <-.
+  Admitted. *)
+
+  
+  (* Lemma runb_state_to_list {s1 A s2 B b2}: 
+    runb s1 A s2 B b2 -> state_to_list_cons A.
+  Proof.
+    move=> H.
+    elim: H; clear.
+    - move=> s1 s2 A B C b + _.
+      apply: expandedb_done_state_to_list.
+    - move=> s s' r A B C D b1 b2 b3 HA HB HC IH ?; subst.
+      move: HA HB; clear.
+      apply expandedb_fail_state_to_list.
+  Qed. *)
+
+  (* Lemma expandedb_fail_state_to_list {s A B b1 s' C}:
+    expandedb s A (Failed B) b1 -> next_alt s B = Some (s', C) -> 
+      state_to_list A l = x :: xs -> 
+        exists y ys, xs = y ys /\ nur p s' x xs 
+  Proof.
+    remember (Failed _) as f eqn:Hf => H.
+    elim: H B Hf => //; clear.
+    - move=> s A B HA ? [] <-.
+  Admitted. *)
 
   Lemma expand_done {s A s1 B}:
     expand s A = Solved s1 B ->
       forall l,
         exists r1,
-          (nur' r1 A l s) /\ state_to_list (clean_success B) l = r1.
+          (nur' r1 A l s s1) /\ state_to_list (clean_success B) l = r1.
   Proof.
     move=> H l .
     have [sA sB] := expand_solved_success H.
     (* move=>[]<- H1. *)
     eexists; split; last first.
-    apply: state_to_list_eq_clean sB sA _.
-    symmetry.
-    apply: expand_solved_state_to_list_same  H.
+      apply: state_to_list_eq_clean sB sA _.
+      symmetry.
+      apply: expand_solved_state_to_list_same  H.
     rewrite /nur' => x xs + p.
     rewrite (success_state_to_list sA) => -[<-<-].
-    eexists; apply: StopE.
+    rewrite (expand_solved_same_subst H).
+    apply: StopE.
   Qed.
-
-  Definition get_subst R :=
-    match R with
-    | Solved s _ => s
-    | Expanded s _ => s
-    | CutBrothers s _ => s
-    | Failure _ => empty
-    end.
-  
-  Lemma wwww {s1 A r}: 
-    expand s1 A = r -> is_fail r == false -> 
-      forall {s2 C b}, expandedb (get_subst r) (get_state r) (Done s2 C) b ->
-        forall {l}, exists x xs, state_to_list (get_state r) l = x :: xs.
-  Proof.
-    elim: A s1 r => //; try by move=>s1 r <- /=; do 2 eexists.
-    - move=>/=p [|t]//s1 r <- _/=.
-        by do 2 eexists.
-      rewrite /big_or/F.
-      case X: select => [|[s3 r2] ys]/=.
-        inversion 1; subst => //.
-      inversion 1; subst => //.
-    - move=> A HA s B HB s1 []//s3 D + _.
-      - move=> /simpl_expand_or_expanded[].
-          move=>[A2[dA[HA2->]]]/=.
-          move=> s2 E b H.
-          have:= expanded_same_structure (ex_intro _ _ H).
-          case: E H => // A' s' B'/= + /and3P[/eqP ? _ _]; subst.
-          move=> H.
-          have:= expanded_or_complete_left H.
-          move=>[].
-            move=>[dA2 [b' [H1 ?]]] l; subst.
-            have /= := HA _ _ HA2 isT _ _ _ H1 (state_to_list B l ++ l).
-            move=> [y [ys]] ->/=.
-            by do 2 eexists.
-          move=> [-> [b1 H1]] l.
-          rewrite state_to_list_dead/=.
-          inversion H1; subst.
-          - have /= := HB _ _ H6 isT; admit.
-          - have /= := HB _ _ H0 isT _ _ _ H2.
-  Admitted.
 
   Lemma runExpandedbDone {s s' A B b}:
     expandedb s A (Done s' B) b ->
     forall l,
-    exists r1,
-      (nur' r1 A l s) /\ state_to_list (clean_success B) l = r1.
+      exists r1,
+        (nur' r1 A l s s') /\ state_to_list (clean_success B) l = r1.
   Proof.
     remember (Done _ _) as d eqn:Hd => H.
     elim: H s' B Hd => //; clear.
     - move=> s s' A A' + s1 B [??]; subst.
       apply: expand_done.
     - move=> s s' r A B b H1 H2 IH s1 C ? l; subst.
-      have := IH _ _ erefl l.
+      have {IH} := IH _ _ erefl l.
       rewrite /nur'.
       move=> [r1 [H3 H4]].
-      exists r1; split => // x xs H p.
-      clear IH.
+      have [x [xs]] := expandedb_done_state_to_list H2 l.
+      move=>{}/H3 H3.
+      exists r1; split => // w ws H p.
+      have {}H3 := H3 p.
       admit.
     - move=> s s' r A B b H1 H2 IH s1 C ? l; subst.
-      have := IH _ _ erefl l.
+      have {IH} := IH _ _ erefl l.
       rewrite /nur'.
       move=> [r1 [H3 H4]].
-      exists r1; split => // x xs H p.
-      clear IH.
+      have [x [xs]] := expandedb_done_state_to_list H2 l.
+      move=>{}/H3 H3.
+      exists r1; split => // w ws H p.
+      have {}H3 := H3 p.
       admit.
   Admitted.
 
-  (* Lemma xxx {s B}: next_alt s B = None-> state_to_list A x = [::].  *)
-
-  Lemma failed_state_to_list {B}:
-    failed B = false ->
-    forall{l}, exists x xs, state_to_list B l = x :: xs.
-  Proof.
-    elim: B => //; try by move=> /=; do 2 eexists.
-    - by move=> /= _ []; do 2 eexists.
-    - move=> A HA s B HB/=.
-      case: ifP => /eqP.
-        move=>-> H l.
-        rewrite state_to_list_dead.
-        by apply: HB.
-      move=> dA fA l.
-      have:= HA fA ((state_to_list B l ++ l)).
-      by move=>[x[xs]]->; do 2 eexists.
-    - move=> A HA B0 _ B HB /=.
-      case fA: failed => //= + l.
-      have [x [xs]]:= HA fA l.
-      move=>->/=.
-  Abort.
-
-  Lemma fff {s B s' C}: 
-    next_alt s B = Some (s', C) ->
-      forall {l}, exists x xs, state_to_list C l = x :: xs.
-  Proof.
-    elim: B s C s' => //.
-    - move=> A HA s B HB s1 C s'.
-      move=> /=.
-      case: ifP => /eqP.
-        move=>->; case X: next_alt => [[s2 D]|]//.
-        move=>[_<-]/=l; rewrite state_to_list_dead/=.
-        apply: HB X _.
-      move=> dA.
-      case X: next_alt => [[s2 D]|]//.
-        move=>[_ <-]/=l.
-        have:= HA _ _ _ X (state_to_list B l ++ l).
-        move=>[x[xs]]->/=.
-        by do 2 eexists.
-      case: ifP => /eqP// dB.
-      case: ifP => fB.
-        case Y: next_alt => [[s2 D]|]//.
-        move=>[_<-]/=l; rewrite state_to_list_dead/=.
-        by apply: HB Y _.
-      move=>[_<-]l/=.
-      rewrite state_to_list_dead/=.
-    Abort.
-
-
-  Lemma zzzzz {s A B b1}:
+  Lemma xxxx {p s A B b1 l x y ys s' s2 r1}:
     expandedb s A (Failed B) b1 ->
-      forall {x xs l}, state_to_list A l = x :: xs ->
-        forall {s' C}, next_alt s B = Some (s', C) ->
-          state_to_list C l = x :: xs.
+      state_to_list A l = x :: (y::ys) ->
+          nur p s' y ys s2 r1 -> nur p s x (y::ys) s2 r1.
+  Admitted.
+
+  Lemma rrrr {s A B s' C l x xs}:
+    expand s A = Failure B ->
+      next_alt s B = Some (s', C) -> state_to_list A l = x :: xs -> state_to_list C l = xs.
+  Proof.
+    elim: A s B s' C l x xs => //.
+    - move=> s B s' C l x xs[<-]//.
+    - move=> p [|t]//.
+    - move=> A HA s B HB s1 C s2 D l x xs.
+      move=>/simpl_expand_or_fail[].
+        move=>[A'[dA[HA'->]]]/=; clear HB.
+        have /= dA':= expand_not_dead dA HA'.
+        case: ifP => /eqP// _.
+        case X: next_alt => [[s3 E]|].
+          move=>[_<-]/=.
+          case Y: state_to_list => [|y ys].
+            admit.
+          have:= HA _ _ _ _ _ _ _ HA' X Y.
+          by move=>->[].
+        case: ifP => /eqP//dB.
+        case: ifP => fB//.
+          case: next_alt => [[s3 E]|]//.
+          move=>[_<-]/=.
+          rewrite state_to_list_dead/=.
+          case Y: state_to_list => [|y ys]/=.
+            admit.
+          move=>[] _ H.
+
+      move=>
+
+  Lemma zzzz {s A B b1 l x xs s' C}:
+    expandedb s A (Failed B) b1 ->
+      next_alt s B = Some (s', C) ->
+        state_to_list A l = x :: xs ->
+          state_to_list C l = xs.
   Proof.
     remember (Failed _) as f eqn:Hf => H.
-    elim: H B Hf => //; clear.
-    - move=> s A B H B1 [<-] x xs l H1 s' C H2.
-  Abort.
+    elim: H B l x xs s' C Hf; clear => //.
+    - move=> s A B + ? l x xs s' C[<-].
+      clear.
 
-  (* Lemma titi {s C r b2 l}: runb s C r b2 -> 
-    exists x xs, state_to_list C l = x :: xs.
-  Proof.
-    move=> H.
-    elim: H l; clear.
-    - move=> s s' A B C b H _ l.
-      admit.
-    - move=> s s' r A B C b1 b2 b3 HA HB HC IH ? l; subst.
-  Abort. *)
+
+
+  Admitted.
+
 
   Lemma runElpiP: forall A, runElpi A.
   Proof.
@@ -474,13 +502,19 @@ Module Nur (U : Unif).
     elim: H; clear.
     + move=>  s s' A B C b + ->/=.
       apply: runExpandedbDone.
-    + move=> s s' r A B C D b1 b2 b3 HA HB HC IH ? l; subst.
-      have := IH l.
+    + move=> s s' s2 A B C D b1 b2 b3 HA HB HC IH ? l; subst.
+      have {IH} := IH l.
       rewrite /nur'.
       move=> [r1 [H1 H2]].
       exists r1; split => // x xs H p.
-      clear IH.
-      admit.
-  Admitted.
+      have:= next_alt_state_to_list HB.
+      move=> /(_ l) [y [ys H3]].
+      have {}H1:= H1 _ _ H3 p.
+      rewrite /state_to_list_cons.
+      have := zzzz HA HB H.
+      rewrite H3 => ?; subst.
+      apply: xxxx HA H H1.
+  Qed.
+  Print Assumptions runElpiP.
 End Nur.
 
